format-version: 1.2
date: 2025-04-21 22:00
saved-by: lukas
default-namespace: TO
ontology: TO

[Term]
id: TO:0000001
name: Taro ontology root
def: "Proportion of stakes germinated scored one month after planting." [CO:curators]

[Term]
id: TO:0000002
name: Agronomic
def: "Agronomic traits" []
is_a: TO:0000001 ! Taro ontology root

[Term]
id: TO:0000003
name: Biotic stress
def: "Biotic stress" []
is_a: TO:0000001 ! Taro ontology root

[Term]
id: TO:0000004
name: Taro leaf blight
is_a: TO:0000003 ! Biotic stress

[Term]
id: TO:0000005
name: Taro leaf blight severity
synonym: "TLBs" []
def: "Visual severity rating of plants infected with taro leaf blight caused by oomycete Phytophthora colocasiae. Evaluation in Trials. Visual scoring based on a scale from 1-5" []
relationship: variable_of: TO:0000004 ! Taro leaf blight

[Term]
id: TO:0000005
name: Taro leaf blight incidence
synonym: "TLBi" []
def: "Proportion of plants within a plot showing symptoms of taro leaf blight. Evaluation in Trials. Proportion of plants within a plot showing symptoms of taro leaf blight" []
relationship: variable_of: TO:0000004 ! Taro leaf blight

[Term]
id: TO:0000006
name: Plant vigour trait
is_a: TO:0000002 ! Agronomic

[Term]
id: TO:0000007
name: Plant vigour
synonym: "VIG" []
def: "A qualitative trait indicating the plant vigour, visual rating. A qualitative trait indicating the plant vigour, visual rating at the scale of 3,5 and 7" []
relationship: variable_of: TO:0000006 ! Plant vigour

[Term]
id: TO:0000008
name: Plant height term
is_a: TO:0000002 ! Agronomic

[Term]
id: TO:0000009
name: Plant height
synonym: "PLT HT" []
def: "Vertical height of plants from the ground to top of the canopy measured in centimeter (cm) or meters (m)	Evaluation in Trials	Agronomic	Measured as height from ground level to the top of canopy at harvest" []
relationship: variable_of: TO:0000008 ! Plant height term

[Term]
id: TO:0000010
name: corms/plot
is_a: TO:0000002 ! Agronomic

[Term]
id: TO:0000011
name: Number of corms/plot
synonym: "CORM NO"
def: "Is a count of the number of corms harvested per plot, Counting the number of corms during harvest" []
relationship: variable_of: TO:0000010 ! corms/plot

[Term]
id: TO:0000012
name: cormels/plot
is_a: TO:0000002 ! Agronomic

[Term]
id: TO:0000013
name: Number of cormels/plot
synonym: "CORMEL NO" []
def: "Is a count of the number of cormels harvested per plot. Counting the number of cormel during harvest" []
relationship: variable_of TO:0000012 ! cormels/plot

[Term]
id: TO:0000014
name: Number of stolons
is_a: TO:0000002 ! Agronomic

[Term]
id: TO:0000015
name: Number of stolons/plot
synonym: "STOLON NO" []
def: "Is a count of the number of stolons harvested per plot. Evaluation in Trials. Method: Counting the number of stolons during harvest" []
relationship: variable_of TO:0000014 ! Number of stolons/plot

[Term]
id: TO:0000016
name: Corm yield
is_a: TO:0000002 ! Agronomic

[Term]
id: TO:0000017
name: Corm yield (g/plot)
synonym: "CORM YLD" []
def: "Weight of corm from a unit plot Evaluation in Trials. Method: Weighing the corms per plot" []
relationship: variable_of TO:0000016 ! Corm yield

[Term]
id: TO:0000018
name: Cormel yield
is_a: TO:0000002 ! Agronomic

[Term]
id: TO:0000019
name: Cormel yield (g/plot)
synonym: "CORMEL YLD" []
def: "Weight of cormel from a unit plot. Method: Weighing the cormels per plot" []

[Term]
id: TO:0000020
name: Total tuber yield
is_a: TO:0000002 ! Agronomic

[Term]
id: TO:0000021
name: Total tuber yield (g/plot)
synonym: "TTW" []
def: "Weight of tuber (corms,cormels and stolons) from a unit plot. Method: Weighing the total tubers per plot" []
relationship: variable_of TO:0000020 ! Total tuber yield

[Term]
id: TO:0000022
name: Biomass
is_a: TO:0000002 ! Agronomic

[Term]
id: TO:0000023
name: Biomass (g/plot)
synonym: "BIOMASS" []
def: "BIOMASS Total plant mass (stem, leaves and petiole) above ground. Total weight of leaf, petiole and stem per plot" []
relationship: variable_of: TO:0000022 ! Biomass

[Term]
id: TO:0000024
name: Harvest Index
is_a: TO:0000002 ! Agronomic

[Term]
id: TO:0000025
name: Harvest Index Proportion
synonym: "HI" []
def: "Proportion of tuber yield over total biomass yield, expressed as a percentage. Method: Ratio between the tuber yield and the total biomass" []

[Term]
id: TO:0000026
name: Number of plant stands harvested
is_a: TO:0000002 ! Agronomic

[Term]
id: TO:0000027
name: Number of plants in a plot at harvest
synonym: "HARVESTED NO" []
def: "Number of plants in a plot at harvest. Method: Count number of plants harvested per plot"
relationship: variable_of TO:0000026 ! Nubmer of plant stands harvested




